theories/Notations.v
@@ -1,5 +1,5 @@
 (** * LogRel.Notations: notations for conversion, typing and the logical relations. *)
-From LogRel Require Import Utils BasicAst Context.
+From LogRel Require Import Utils BasicAst Context LContexts.
 From LogRel.AutoSubst Require Import Ast.
 
 (** We have four families of definitions: the declarative ones (tagged de), the algorithmic ones (tagged al), and the bundled ones, which package an algorithmic typing derivation with its preconditions (tagged bn).
@@ -22,166 +22,166 @@ Close Scope declarative_scope.
 Open Scope typing_scope.
 
 (** ** Typing *)
-Class WfContext (ta : tag) := wf_context : context -> Set.
-Class WfType (ta : tag) := wf_type : context -> term -> Set.
-Class Typing (ta : tag) := typing : context -> term -> term -> Set.
-Class Inferring (ta : tag) := inferring : context -> term -> term -> Set.
-Class InferringRed (ta : tag) := infer_red : context -> term -> term -> Set.
-Class Checking (ta : tag) := check : context -> term -> term -> Set.
-Class TypeNe (ta : tag) := type_ne : context -> term -> Set.
-Class TypeNf (ta : tag) := type_nf : context -> term -> Set.
-Class TermNe (ta : tag) := term_ne : context -> term -> term -> Set.
-Class TermNf (ta : tag) := term_nf : context  -> term -> term -> Set.
-Class ConvType (ta : tag) := conv_type : context  -> term -> term -> Set.
+Class WfContext (ta : tag) := wf_context : wfLCon -> context -> Set.
+Class WfType (ta : tag) := wf_type : wfLCon -> context -> term -> Set.
+Class Typing (ta : tag) := typing : wfLCon -> context -> term -> term -> Set.
+Class Inferring (ta : tag) := inferring : wfLCon -> context  -> term -> term -> Set.
+Class InferringRed (ta : tag) := infer_red : wfLCon -> context  -> term -> term -> Set.
+Class Checking (ta : tag) := check : wfLCon -> context  -> term -> term -> Set.
+Class TypeNe (ta : tag) := type_ne : wfLCon -> context  -> term -> Set.
+Class TypeNf (ta : tag) := type_nf : wfLCon -> context  -> term -> Set.
+Class TermNe (ta : tag) := term_ne : wfLCon -> context  -> term -> term -> Set.
+Class TermNf (ta : tag) := term_nf : wfLCon -> context  -> term -> term -> Set.
+Class ConvType (ta : tag) := conv_type : wfLCon -> context  -> term -> term -> Set.
 Class ConvTypeRed (ta : tag) :=
-  conv_type_red : context  -> term -> term -> Set.
+  conv_type_red : wfLCon -> context  -> term -> term -> Set.
 Class ConvTerm (ta : tag) :=
-  conv_term : context  -> term -> term -> term -> Set.
+  conv_term : wfLCon -> context  -> term -> term -> term -> Set.
 Class ConvTermRed (ta : tag) :=
-  conv_term_red : context  -> term -> term -> term -> Set.
-Class ConvNeu (ta : tag) := conv_neu : context  -> term -> term -> term -> Set.
+  conv_term_red : wfLCon -> context  -> term -> term -> term -> Set.
+Class ConvNeu (ta : tag) := conv_neu : wfLCon -> context  -> term -> term -> term -> Set.
 Class ConvNeuRed (ta : tag) :=
-  conv_neu_red : context  -> term -> term -> term -> Set.
+  conv_neu_red : wfLCon -> context  -> term -> term -> term -> Set.
 Class ConvNeuConv (ta : tag) :=
-  conv_neu_conv : context  -> term -> term -> term -> Set.
+  conv_neu_conv : wfLCon -> context  -> term -> term -> term -> Set.
 
 (** The context Γ is well-formed *)
-Notation "[ |- Γ ]" := (wf_context Γ)
-  (at level 0, Γ at level 50, only parsing) : typing_scope.
-Notation "[ |-[ ta  ] Γ ]" := (wf_context (ta := ta) Γ)
-  (at level 0, ta, Γ at level 50) : typing_scope.
+Notation "[ |- Γ ]< l >" := (wf_context l Γ)
+  (at level 0, Γ, l at level 50, only parsing) : typing_scope.
+Notation "[ |-[ ta  ] Γ ]< l >" := (wf_context (ta := ta) l Γ)
+  (at level 0, ta, Γ, l at level 50) : typing_scope.
 (** The contexts Γ and Δ are convertible *)
-Reserved Notation "[ |- Γ ≅ Δ ]" (at level 0, Γ, Δ at level 50).
-Reserved Notation "[ |-[ ta  ] Γ ≅ Δ ]" (at level 0, ta, Γ, Δ at level 50).
+Reserved Notation "[ |- Γ ≅ Δ ]< l >" (at level 0, Γ, l, Δ at level 50).
+Reserved Notation "[ |-[ ta  ] Γ ≅ Δ ]< l >" (at level 0, ta, Γ, l, Δ at level 50).
 (** The type A is well-formed in Γ *)
-Notation "[ Γ |- A ]" := (wf_type Γ A)
-  (at level 0, Γ, A at level 50, only parsing) : typing_scope.
-Notation "[ Γ |-[ ta  ] A ]" := (wf_type (ta := ta) Γ A)
-  (at level 0, ta, Γ, A at level 50) : typing_scope.
+Notation "[ Γ |- A ]< l >" := (wf_type l Γ A)
+  (at level 0, Γ, l, A at level 50, only parsing) : typing_scope.
+Notation "[ Γ |-[ ta  ] A ]< l >" := (wf_type (ta := ta) l Γ A)
+  (at level 0, ta, Γ, l, A at level 50) : typing_scope.
 
 (** The term t has type A in Γ *)
-Notation "[ Γ |- t : A ]" := (typing Γ A t)
-  (at level 0, Γ, t, A at level 50, only parsing) : typing_scope.
-Notation "[ Γ |-[ ta  ] t : A ]" :=
-  (typing (ta := ta) Γ A t) (at level 0, ta, Γ, t, A at level 50) : typing_scope.
+Notation "[ Γ |- t : A ]< l >" := (typing l Γ A t)
+  (at level 0, Γ, l, t, A at level 50, only parsing) : typing_scope.
+Notation "[ Γ |-[ ta  ] t : A ]< l >" :=
+  (typing (ta := ta) l Γ A t) (at level 0, ta, Γ, l, t, A at level 50) : typing_scope.
 
-Notation "Nf[ Γ |- A ]" := (type_nf Γ A)
-  (at level 0, Γ, A at level 50, only parsing) : typing_scope.
-Notation "Nf[ Γ |-[ ta  ] A ]" := (type_nf (ta := ta) Γ A)
-  (at level 0, Γ, A at level 50) : typing_scope.
-Notation "Ne[ Γ |- A ]" := (type_ne Γ A)
-  (at level 0, Γ, A at level 50, only parsing) : typing_scope.
-Notation "Ne[ Γ |-[ ta  ] A ]" := (type_ne (ta := ta) Γ A)
-  (at level 0, Γ, A at level 50) : typing_scope.
-Notation "Nf[ Γ |- t : A ]" := (term_nf Γ A t)
-  (at level 0, Γ, t, A at level 50, only parsing) : typing_scope.
-Notation "Nf[ Γ |-[ ta  ] t : A ]" := (term_nf (ta := ta) Γ A t)
-  (at level 0, Γ, t, A at level 50) : typing_scope.
-Notation "Ne[ Γ |- t : A ]" := (term_ne Γ A t)
-  (at level 0, Γ, t, A at level 50, only parsing) : typing_scope.
-Notation "Ne[ Γ |-[ ta  ] t : A ]" := (term_ne (ta := ta) Γ A t)
-  (at level 0, Γ, t, A at level 50) : typing_scope.
+Notation "Nf[ Γ |- A ]< l >" := (type_nf l Γ A)
+  (at level 0, Γ, l, A at level 50, only parsing) : typing_scope.
+Notation "Nf[ Γ |-[ ta  ] A ]< l >" := (type_nf (ta := ta) l Γ A)
+  (at level 0, Γ, l, A at level 50) : typing_scope.
+Notation "Ne[ Γ |- A ]< l >" := (type_ne l Γ A)
+  (at level 0, Γ, l, A at level 50, only parsing) : typing_scope.
+Notation "Ne[ Γ |-[ ta  ] A ]< l >" := (type_ne (ta := ta) l Γ A)
+  (at level 0, Γ, l, A at level 50) : typing_scope.
+Notation "Nf[ Γ |- t : A ]< l >" := (term_nf l Γ A t)
+  (at level 0, Γ, l, t, A at level 50, only parsing) : typing_scope.
+Notation "Nf[ Γ |-[ ta  ] t : A ]< l >" := (term_nf (ta := ta) l Γ A t)
+  (at level 0, Γ, l, t, A at level 50) : typing_scope.
+Notation "Ne[ Γ |- t : A ]< l >" := (term_ne l Γ A t)
+  (at level 0, Γ, l, t, A at level 50, only parsing) : typing_scope.
+Notation "Ne[ Γ |-[ ta  ] t : A ]< l >" := (term_ne (ta := ta) l Γ A t)
+  (at level 0, Γ, l, t, A at level 50) : typing_scope.
 (** The term t checks against type A in Γ *)
-Notation "[ Γ |- t ◃ A ]" := (check Γ A t)
-  (at level 0, Γ, t, A at level 50, only parsing) : typing_scope.
-Notation "[ Γ |-[ ta  ] t ◃ A ]" :=
-  (check (ta := ta) Γ A t) (at level 0, ta, Γ, t, A at level 50) : typing_scope.
+Notation "[ Γ |- t ◃ A ]< l >" := (check l Γ A t)
+  (at level 0, Γ, l, t, A at level 50, only parsing) : typing_scope.
+Notation "[ Γ |-[ ta  ] t ◃ A ]< l >" :=
+  (check (ta := ta) l Γ A t) (at level 0, ta, Γ, l, t, A at level 50) : typing_scope.
 (** The term t infers A in Γ *)
-Notation "[ Γ |- t ▹ A ]" := (inferring Γ A t)
-  (at level 0, Γ, t, A at level 50, only parsing) : typing_scope.
-Notation "[ Γ |-[ ta  ] t ▹ A ]" :=
-  (inferring (ta := ta) Γ A t) (at level 0, ta, Γ, t, A at level 50) : typing_scope.
+Notation "[ Γ |- t ▹ A ]< l >" := (inferring l Γ A t)
+  (at level 0, Γ, l, t, A at level 50, only parsing) : typing_scope.
+Notation "[ Γ |-[ ta  ] t ▹ A ]< l >" :=
+  (inferring (ta := ta) l Γ A t) (at level 0, ta, Γ, l, t, A at level 50) : typing_scope.
 (** The term t infers the reduced A in Γ *)
-Notation "[ Γ |- t ▹h A ]" := (infer_red Γ A t) (at level 0, Γ, t, A at level 50, only parsing) : typing_scope.
-Notation "[ Γ |-[ ta  ] t ▹h A ]" := (infer_red (ta := ta) Γ A t) (at level 0, ta, Γ, t, A at level 50) : typing_scope.
+Notation "[ Γ |- t ▹h A ]< l >" := (infer_red l Γ A t) (at level 0, Γ, l, t, A at level 50, only parsing) : typing_scope.
+Notation "[ Γ |-[ ta  ] t ▹h A ]< l >" := (infer_red (ta := ta) l Γ A t) (at level 0, ta, Γ, l, t, A at level 50) : typing_scope.
 (** Types A and B are convertible in Γ *)
-Notation "[ Γ |- A ≅ B ]" := (conv_type Γ A B)
-  (at level 0, Γ, A, B at level 50, only parsing) : typing_scope.
-Notation "[ Γ |-[ ta  ] A ≅ B ]" := (conv_type (ta := ta) Γ A B)
-  (at level 0, ta, Γ, A, B at level 50) : typing_scope.
+Notation "[ Γ |- A ≅ B ]< l >" := (conv_type l Γ A B)
+  (at level 0, Γ, l, A, B at level 50, only parsing) : typing_scope.
+Notation "[ Γ |-[ ta  ] A ≅ B ]< l >" := (conv_type (ta := ta) l Γ A B)
+  (at level 0, ta, Γ, l, A, B at level 50) : typing_scope.
 (** Types in whnf A and B are convertible in Γ *)
-Notation "[ Γ |- A '≅h' B ]" := (conv_type_red Γ A B) (at level 0, Γ, A, B at level 50, only parsing) : typing_scope.
-Notation "[ Γ |-[ ta  ] A '≅h' B ]" := (conv_type_red (ta := ta) Γ A B) (at level 0, ta, Γ, A, B at level 50) : typing_scope.
+Notation "[ Γ |- A '≅h' B ]< l >" := (conv_type_red l Γ A B) (at level 0, Γ, l, A, B at level 50, only parsing) : typing_scope.
+Notation "[ Γ |-[ ta  ] A '≅h' B ]< l >" := (conv_type_red (ta := ta) l Γ A B) (at level 0, ta, Γ, l, A, B at level 50) : typing_scope.
 (** Terms t and t' are convertible in Γ *)
-Notation "[ Γ |- t ≅ t' : A ]" := (conv_term Γ A t t')
-  (at level 0, Γ, t, t', A at level 50, only parsing) : typing_scope.
-Notation "[ Γ |-[ ta  ] t ≅ t' : A ]" := (conv_term (ta := ta) Γ A t t')
-  (at level 0, ta, Γ, t, t', A at level 50) : typing_scope.
+Notation "[ Γ |- t ≅ t' : A ]< l >" := (conv_term l Γ A t t')
+  (at level 0, Γ, l, t, t', A at level 50, only parsing) : typing_scope.
+Notation "[ Γ |-[ ta  ] t ≅ t' : A ]< l >" := (conv_term (ta := ta) l Γ A t t')
+  (at level 0, ta, Γ, l, t, t', A at level 50) : typing_scope.
 (** Whnfs t and t' are convertible in Γ *)
-Notation "[ Γ |- t '≅h' t' : A ]" := (conv_term_red Γ A t t') (at level 0, Γ, t, t', A at level 50, only parsing) : typing_scope.
-Notation "[ Γ |-[ ta  ] t '≅h' t' : A ]" := (conv_term_red (ta := ta) Γ A t t') (at level 0, ta, Γ, t, t', A at level 50) : typing_scope.
+Notation "[ Γ |- t '≅h' t' : A ]< l >" := (conv_term_red l Γ A t t') (at level 0, Γ, l, t, t', A at level 50, only parsing) : typing_scope.
+Notation "[ Γ |-[ ta  ] t '≅h' t' : A ]< l >" := (conv_term_red (ta := ta) l Γ A t t') (at level 0, ta, Γ, l, t, t', A at level 50) : typing_scope.
 (** Neutral n and n' are convertible in Γ, inferring the type A *)
-Notation "[ Γ |- n ~ n' ▹ A ]" := (conv_neu Γ A n n')
-  (at level 0, Γ, n, n', A at level 50, only parsing) : typing_scope. 
-Notation "[ Γ |-[ ta  ] n ~ n' ▹ A ]" := (conv_neu (ta := ta) Γ A n n')
-  (at level 0, ta, Γ, n, n', A at level 50) : typing_scope.
+Notation "[ Γ |- n ~ n' ▹ A ]< l >" := (conv_neu l Γ A n n')
+  (at level 0, Γ, l, n, n', A at level 50, only parsing) : typing_scope. 
+Notation "[ Γ |-[ ta  ] n ~ n' ▹ A ]< l >" := (conv_neu (ta := ta) l Γ A n n')
+  (at level 0, ta, Γ, l, n, n', A at level 50) : typing_scope.
 (** Neutral n and n' are convertible in Γ, inferring the reduced type A *)
-Notation "[ Γ |- n '~h' n' ▹ A ]" := (conv_neu_red Γ A n n') (at level 0, Γ, n, n', A at level 50, only parsing) : typing_scope.
-Notation "[ Γ |-[ ta  ] n '~h' n' ▹ A ]" := (conv_neu_red (ta := ta) Γ A n n') (at level 0, ta, Γ, n, n', A at level 50) : typing_scope.
+Notation "[ Γ |- n '~h' n' ▹ A ]< l >" := (conv_neu_red l Γ A n n') (at level 0, Γ, l, n, n', A at level 50, only parsing) : typing_scope.
+Notation "[ Γ |-[ ta  ] n '~h' n' ▹ A ]< l >" := (conv_neu_red (ta := ta) l Γ A n n') (at level 0, ta, Γ, l, n, n', A at level 50) : typing_scope.
 (** Neutral n and n' are convertible in Γ at type A *)
-Notation "[ Γ |- n ~ n' : A ]" := (conv_neu_conv Γ A n n')
-  (at level 0, Γ, n, n', A at level 50, only parsing) : typing_scope. 
-Notation "[ Γ |-[ ta  ] n ~ n' : A ]" := (conv_neu_conv (ta := ta) Γ A n n')
-  (at level 0, ta, Γ, n, n', A at level 50) : typing_scope.
+Notation "[ Γ |- n ~ n' : A ]< l >" := (conv_neu_conv l Γ A n n')
+  (at level 0, Γ, l, n, n', A at level 50, only parsing) : typing_scope. 
+Notation "[ Γ |-[ ta  ] n ~ n' : A ]< l >" := (conv_neu_conv (ta := ta) l Γ A n n')
+  (at level 0, ta, Γ, l, n, n', A at level 50) : typing_scope.
 
 (** ** Reductions *)
-Class RedType (ta : tag) := red_ty : context -> term -> term -> Set.
+Class RedType (ta : tag) := red_ty : wfLCon -> context -> term -> term -> Set.
 Class OneStepRedTerm (ta : tag) :=
-  osred_tm : context -> term -> term -> term -> Set.
-Class RedTerm (ta : tag) := red_tm : context -> term -> term -> term -> Set.
+  osred_tm : wfLCon -> context -> term -> term -> term -> Set.
+Class RedTerm (ta : tag) := red_tm : wfLCon -> context -> term -> term -> term -> Set.
 
 (** Term t untyped one-step weak-head reduces to term t' *)
-Reserved Notation "[ t ⇒ t' ]< l >" (at level 0, t, t', l at level 50).
+Reserved Notation "[ t ⇒ t' ]< l >" (at level 0, l, t, t' at level 50).
 (** Term t untyped multi-step weak-head reduces to term t' *)
-Reserved Notation "[ t ⇒* t' ]< l >" (at level 0, t, t', l at level 50).
+Reserved Notation "[ t ⇒* t' ]< l >" (at level 0, l, t, t' at level 50).
 
 (** Type A one-step weak-head reduces to type B in Γ *)
-Reserved Notation "[ Γ |- A ⇒ B ]" (at level 0, Γ, A, B at level 50).
+Reserved Notation "[ Γ |- A ⇒ B ]< l >" (at level 0, Γ, l, A, B at level 50).
 (** Term or type t one-step weak-head reduces to term or type type u as class A in Γ *)
-Reserved Notation "[ Γ |- t ⇒ u ∈ A ]" (at level 0, Γ, t, u, A at level 50).
+Reserved Notation "[ Γ |- t ⇒ u ∈ A ]< l >" (at level 0, Γ, l, t, u, A at level 50).
 (** Term or type t multi-step weak-head reduces to term or type type u as class A in Γ *)
-Reserved Notation "[ Γ |- t ⇒* u ∈ A ]" (at level 0, Γ, t, u, A at level 50).
+Reserved Notation "[ Γ |- t ⇒* u ∈ A ]< l >" (at level 0, Γ, l, t, u, A at level 50).
 (** Term t one-step weak-head reduces to term u at type A in Γ *)
-Notation "[ Γ |- t ⇒ u : A ]" := (osred_tm Γ A t u) (at level 0, Γ, t, u, A at level 50, only parsing) : typing_scope.
-Notation "[ Γ |-[ ta  ] t ⇒ u : A ]" := (osred_tm (ta:=ta) Γ A t u) (at level 0, ta,Γ, t, u, A at level 50) : typing_scope.
+Notation "[ Γ |- t ⇒ u : A ]< l >" := (osred_tm l Γ A t u) (at level 0, Γ, l, t, u, A at level 50, only parsing) : typing_scope.
+Notation "[ Γ |-[ ta  ] t ⇒ u : A ]< l >" := (osred_tm (ta:=ta) l Γ A t u) (at level 0, ta,Γ, t, u, A at level 50) : typing_scope.
 (** Type A multi-step weak-head reduces to type B in Γ *)
-Notation "[ Γ |- A ⇒* B ]" := (red_ty Γ A B) (at level 0, Γ, A, B at level 50, only parsing) : typing_scope.
-Notation "[ Γ |-[ ta  ] A ⇒* B ]" := (red_ty (ta := ta) Γ A B)
-(at level 0, ta, Γ, A, B at level 50) : typing_scope.
+Notation "[ Γ |- A ⇒* B ]< l >" := (red_ty l Γ A B) (at level 0, Γ, l, A, B at level 50, only parsing) : typing_scope.
+Notation "[ Γ |-[ ta  ] A ⇒* B ]< l >" := (red_ty (ta := ta) l Γ A B)
+(at level 0, ta, Γ, l, A, B at level 50) : typing_scope.
 (** Term t multi-step weak-head reduces to term t' at type A in Γ *)
-Notation "[ Γ |- t ⇒* t' : A ]" := (red_tm Γ A t t')
-(at level 0, Γ, t, t', A at level 50, only parsing) : typing_scope.
-Notation "[ Γ |-[ ta  ] t ⇒* t' : A ]" := (red_tm (ta := ta) Γ A t t')
-(at level 0, ta, Γ, t, t', A at level 50) : typing_scope.
+Notation "[ Γ |- t ⇒* t' : A ]< l >" := (red_tm l Γ A t t')
+(at level 0, Γ, l, t, t', A at level 50, only parsing) : typing_scope.
+Notation "[ Γ |-[ ta  ] t ⇒* t' : A ]< l >" := (red_tm (ta := ta) l Γ A t t')
+(at level 0, ta, Γ, l, t, t', A at level 50) : typing_scope.
 (** Set A weak-head normalizes to B in Γ, ie it multi-step reduces to the weak-head normal form B*)
-Reserved Notation "[ Γ |- A ↘ B ]" (at level 0, Γ, A, B at level 50).
-Reserved Notation "[ Γ |-[ ta  ] A ↘ B ]" (at level 0, ta, Γ, A, B at level 50).
+Reserved Notation "[ Γ |- A ↘ B ]< l >" (at level 0, Γ, l, A, B at level 50).
+Reserved Notation "[ Γ |-[ ta  ] A ↘ B ]< l >" (at level 0, ta, Γ, l, A, B at level 50).
 (** Term t weak-head normalizes to u at type A in Γ *)
-Reserved Notation "[ Γ |- t ↘ u : A ]" (at level 0, Γ, t, u, A at level 50).
-Reserved Notation "[ Γ |-[ ta  ] t ↘ u : A ]" (at level 0, ta, Γ, t, u, A at level 50).
+Reserved Notation "[ Γ |- t ↘ u : A ]< l >" (at level 0, Γ, l, t, u, A at level 50).
+Reserved Notation "[ Γ |-[ ta  ] t ↘ u : A ]< l >" (at level 0, ta, Γ, l, t, u, A at level 50).
 
 (** ** Substitutions *)
 
 (** Substitution σ is of type Δ in context Γ*)
-Reserved Notation "[ Γ '|-s' σ : Δ ]" (at level 0, Γ, σ, Δ at level 50).
-Reserved Notation "[ Γ |-[ ta  ']s' σ : Δ ]" (at level 0, ta, Γ, σ, Δ at level 50).
+Reserved Notation "[ Γ '|-s' σ : Δ ]< l >" (at level 0, Γ, l, σ, Δ at level 50).
+Reserved Notation "[ Γ |-[ ta  ']s' σ : Δ ]< l >" (at level 0, ta, Γ, l, σ, Δ at level 50).
 (** Substitutions σ and τ are convertible at types Δ in context Γ *)
-Reserved Notation "[ Γ '|-s' σ ≅ τ : Δ ]" (at level 0, Γ, σ, τ, Δ at level 50).
-Reserved Notation "[ Γ |-[ ta  ']s' σ ≅ τ : Δ ]" (at level 0, ta, Γ, σ, τ, Δ at level 50).
+Reserved Notation "[ Γ '|-s' σ ≅ τ : Δ ]< l >" (at level 0, Γ, l, σ, τ, Δ at level 50).
+Reserved Notation "[ Γ |-[ ta  ']s' σ ≅ τ : Δ ]< l >" (at level 0, ta, Γ, l, σ, τ, Δ at level 50).
 
 (** ** Extra typing conditions *)
 (** Types A and B are well-formed and convertible in Γ *)
-Reserved Notation "[ Γ |- A :≅: B ]" (at level 0, Γ, A, B at level 50).
-Reserved Notation "[ Γ |-[ ta  ] A :≅: B ]" (at level 0, ta, Γ, A, B at level 50).
+Reserved Notation "[ Γ |- A :≅: B ]< l >" (at level 0, Γ, l, A, B at level 50).
+Reserved Notation "[ Γ |-[ ta  ] A :≅: B ]< l >" (at level 0, ta, Γ, l, A, B at level 50).
 (** Terms t and u are well-typed and convertible at type A in Γ *)
-Reserved Notation "[ Γ |- t :≅: u : A ]" (at level 0, Γ, t, u, A at level 50).
-Reserved Notation "[ Γ |-[ ta  ] t :≅: u : A ]" (at level 0, ta, Γ, t, u, A at level 50).
+Reserved Notation "[ Γ |- t :≅: u : A ]< l >" (at level 0, Γ, l, t, u, A at level 50).
+Reserved Notation "[ Γ |-[ ta  ] t :≅: u : A ]< l >" (at level 0, ta, Γ, l, t, u, A at level 50).
 (** Set A and B are well-formed and A weak-head reduces to B in Γ *)
-Reserved Notation "[ Γ |- A :⇒*: B ]" (at level 0, Γ, A, B at level 50).
-Reserved Notation "[ Γ |-[ ta  ] A :⇒*: B ]" (at level 0, ta, Γ, A, B at level 50).
+Reserved Notation "[ Γ |- A :⇒*: B ]< l >" (at level 0, Γ, l, A, B at level 50).
+Reserved Notation "[ Γ |-[ ta  ] A :⇒*: B ]< l >" (at level 0, ta, Γ, l, A, B at level 50).
 (** Terms t and u have type A in Γ and t weak-head reduces to u *)
-Reserved Notation "[ Γ |- t :⇒*: u : A ]" (at level 0, Γ, t, u, A at level 50).
-Reserved Notation "[ Γ |-[ ta  ] t :⇒*: u : A ]" (at level 0, ta, Γ, t, u, A at level 50).
+Reserved Notation "[ Γ |- t :⇒*: u : A ]< l >" (at level 0, Γ, l, t, u, A at level 50).
+Reserved Notation "[ Γ |-[ ta  ] t :⇒*: u : A ]< l >" (at level 0, ta, Γ, l, t, u, A at level 50).
 
 (** ** Weakenings *)
 (** Well-formed weakening *)
@@ -192,92 +192,92 @@ Reserved Notation "ρ ∘w ρ'" (at level 50).
 
 (** ** Logical relation *)
 (** The universe is reducible in Γ, according to the kit K *)
-Reserved Notation "[ K | Γ ||-U ]" (at level 0, K, Γ at level 50).
+Reserved Notation "[ K | Γ ||-U ]< l >" (at level 0, K, Γ, l at level 50).
 (** The type A is reducible as a Π type in Γ according to the kit K *)
-Reserved Notation "[ K | Γ ||-Π A ]" (at level 0, K, Γ, A at level 50).
+Reserved Notation "[ K | Γ ||-Π A ]< l >" (at level 0, K, Γ, l, A at level 50).
 (** The type A is reducible in Γ, according to the kit K *)
-Reserved Notation "[ K | Γ ||- A ]"  (at level 0, K, Γ, A at level 50).
+Reserved Notation "[ K | Γ ||- A ]< l >"  (at level 0, K, Γ, l, A at level 50).
 (** The types A and B are reducibly convertible in Γ, given the proof R than A is reducible, according to the kit K*)
-Reserved Notation "[ K | Γ ||- A ≅ B | R ]" (at level 0, K, Γ, A, B, R at level 50).
+Reserved Notation "[ K | Γ ||- A ≅ B | R ]< l >" (at level 0, K, Γ, l, A, B, R at level 50).
 (** The term t is reducible at type A in Γ, given the proof R than A is reducible, according to the kit K *)
-Reserved Notation "[ K | Γ ||- t : A | R ]"  (at level 0, K, Γ, t, A, R at level 50).
+Reserved Notation "[ K | Γ ||- t : A | R ]< l >"  (at level 0, K, Γ, l, t, A, R at level 50).
 (** The terms t and u are reducibly convertible at type A in Γ, given the proof R than A is reducible, according to the kit K *)
-Reserved Notation "[ K | Γ ||- t ≅ u : A | R ]" (at level 0, K, Γ, t, u, A, R at level 50).
+Reserved Notation "[ K | Γ ||- t ≅ u : A | R ]< l >" (at level 0, K, Γ, l, t, u, A, R at level 50).
 
 (** The types A and B are reducibly equal in Γ, according to the pack P for Γ and A *)
-Reserved Notation "[ P | Γ ||- A ≅ B ]" (at level 0, P, Γ, A, B at level 50).
+Reserved Notation "[ P | Γ ||- A ≅ B ]< l >" (at level 0, P, Γ, l, A, B at level 50).
 (** The term t is reducible at type A in Γ, according to the pack P *)
-Reserved Notation "[ P | Γ ||- t : A ]" (at level 0, P, Γ, t, A at level 50).
+Reserved Notation "[ P | Γ ||- t : A ]< l >" (at level 0, P, Γ, l, t, A at level 50).
 (** The terms t and u are reducibly equal at type A in Γ, according to the pack P *)
-Reserved Notation "[ P | Γ ||- t ≅ u : A ]" (at level 0, P, Γ, t, u, A at level 50).
+Reserved Notation "[ P | Γ ||- t ≅ u : A ]< l >" (at level 0, P, Γ, l, t, u, A at level 50).
 
 (** Set level l is (strictly) smaller than type level l' *)
 Reserved Notation "l << l'" (at level 70, l' at next level).
 
 (** A is reducible as a neutral in Γ *)
-Reserved Notation "[ Γ ||-ne A ]" (at level 0, Γ, A at level 50).
+Reserved Notation "[ Γ ||-ne A ]< l >" (at level 0, Γ, l, A at level 50).
 (** Set B is reducibly convertible to type A in Γ, given the proof neA that A is reducible as neutral *)
-Reserved Notation "[ Γ ||-ne A ≅ B | neA ]" (at level 0, Γ, A, B, neA at level 50).
+Reserved Notation "[ Γ ||-ne A ≅ B | neA ]< l >" (at level 0, Γ, l, A, B, neA at level 50).
 (** Term t is reducible at type A in Γ, given the proof neA that A is reducible as neutral *)
-Reserved Notation "[ Γ ||-ne t : A | neA ]" (at level 0, Γ, t, A, neA at level 50).
+Reserved Notation "[ Γ ||-ne t : A | neA ]< l >" (at level 0, Γ, l, t, A, neA at level 50).
 (** Terms t and u are reducibly convertible at type A in Γ, given the proof neA that A is reducible as neutral *)
-Reserved Notation "[ Γ ||-ne t ≅ u : A | neA ]" (at level 0, Γ, t, u, A at level 50).
+Reserved Notation "[ Γ ||-ne t ≅ u : A | neA ]< l >" (at level 0, Γ, l, t, u, A at level 50).
 
 (** The type U is reducible in Γ at level k *)
-Reserved Notation "[ Γ ||-U k ]" (at level 0, Γ, k at level 50).
+Reserved Notation "[ Γ ||-U k ]< l >" (at level 0, Γ, l, k at level 50).
 (** The type B is reducibly convertible to U *)
-Reserved Notation "[ Γ ||-U≅ B ]" (at level 0, Γ, B at level 50).
+Reserved Notation "[ Γ ||-U≅ B ]< l >" (at level 0, Γ, l, B at level 50).
 (** The term t is reducible at the universe U, given the proof R that the universe is reducible and the kits rec at lower levels *)
-Reserved Notation "[ rec | Γ ||-U t :U | R ]" (at level 0, rec, Γ, t, R at level 50).
+Reserved Notation "[ rec | Γ ||-U t :U | R ]< l >" (at level 0, rec, Γ, l, t, R at level 50).
 (** The terms t and u are reducibly convertible at the universe U, given the same *)
-Reserved Notation "[ rec | Γ ||-U t ≅ u :U | R ]" (at level 0, rec, Γ, t, u, R at level 50).
+Reserved Notation "[ rec | Γ ||-U t ≅ u :U | R ]< l >" (at level 0, rec, Γ, l, t, u, R at level 50).
 
 
 (** The type A has the packs of a reducible Π type in Γ *)
-Reserved Notation "[ Γ ||-Πd A ]" (at level 0, Γ, A at level 50).
+Reserved Notation "[ Γ ||-Πd A ]< l >" (at level 0, Γ, l, A at level 50).
 (** The type B is reducibly convertible to A in Γ, given the reducibility pack ΠA *)
-Reserved Notation "[ Γ ||-Π A ≅ B | ΠA ]" (at level 0, Γ, A, B, ΠA at level 50).
+Reserved Notation "[ Γ ||-Π A ≅ B | ΠA ]< l >" (at level 0, Γ, l, A, B, ΠA at level 50).
 (** The term t is reducible at type A in Γ, given the reducibility pack ΠA *)
-Reserved Notation "[ Γ ||-Π t : A | ΠA ]" (at level 0, Γ, t, A, ΠA at level 50).
+Reserved Notation "[ Γ ||-Π t : A | ΠA ]< l >" (at level 0, Γ, l, t, A, ΠA at level 50).
 (** The terms t and u are reducibly convertible at type A in Γ, given the reducibility pack ΠA *)
-Reserved Notation "[ Γ ||-Π t ≅ u : A | ΠA ]" (at level 0, Γ, t, u, A, ΠA at level 50).
+Reserved Notation "[ Γ ||-Π t ≅ u : A | ΠA ]< l >" (at level 0, Γ, l, t, u, A, ΠA at level 50).
 
 (** The universe is reducible in Γ at level l *)
-Reserved Notation "[ Γ ||-< k >U]" (at level 0, Γ, k at level 50).
+Reserved Notation "[ Γ ||-< k >U]< l >" (at level 0, Γ, l, k at level 50).
 (** The type A is reducible as a Π type in Γ at level l *)
-Reserved Notation "[ Γ ||-< k >Π  A ]" (at level 0, Γ, k, A at level 50).
+Reserved Notation "[ Γ ||-< k >Π  A ]< l >" (at level 0, Γ, l, k, A at level 50).
 (** The type A is reducible in Γ at level l *)
-Reserved Notation "[ Γ ||-< k >  A ]" (at level 0, Γ, k, A at level 50).
+Reserved Notation "[ Γ ||-< k >  A ]< l >" (at level 0, Γ, l, k, A at level 50).
 (** The types A and B are reducibly convertible in Γ at level l, given the proof R that A is reducible *)
-Reserved Notation "[ Γ ||-< k >  A ≅ B | R ]" (at level 0, Γ, k, A, B, R at level 50).
+Reserved Notation "[ Γ ||-< k >  A ≅ B | R ]< l >" (at level 0, Γ, l, k, A, B, R at level 50).
 (** The term t is reducible at type A and level l in Γ, given the proof R that A is reducible *)
-Reserved Notation "[ Γ ||-< k >  t : A | R ]" (at level 0, Γ, k, t, A, R at level 50).
+Reserved Notation "[ Γ ||-< k >  t : A | R ]< l >" (at level 0, Γ, l, k, t, A, R at level 50).
 (** The terms t and u are reducibly convertible at type A and level l in Γ, given the proof R that A is reducible *)
-Reserved Notation "[ Γ ||-< k > t ≅ u : A | R ]" (at level 0, Γ, k, t, u, A, R at level 50).
+Reserved Notation "[ Γ ||-< k > t ≅ u : A | R ]< l >" (at level 0, Γ, l, k, t, u, A, R at level 50).
 
 (** The type A is reducible in Γ at level 0*)
-Reserved Notation "[ Γ ||-<0>  A ]" (at level 0, Γ, A at level 50).
+Reserved Notation "[ Γ ||-<0>  A ]< l >" (at level 0, Γ, l, A at level 50).
 (** The types A and B are reducibly convertible in Γ at level 0, given the proof R that A is reducible *)
-Reserved Notation "[ Γ ||-<0>  A ≅ B | R ]" (at level 0, Γ, A, B, R at level 50).
+Reserved Notation "[ Γ ||-<0>  A ≅ B | R ]< l >" (at level 0, Γ, l, A, B, R at level 50).
 (** The term t is reducible at type A and level 0 in Γ, given the proof R that A is reducible *)
-Reserved Notation "[ Γ ||-<0>  t : A | R ]" (at level 0, Γ, t, A, R at level 50).
+Reserved Notation "[ Γ ||-<0>  t : A | R ]< l >" (at level 0, Γ, l, t, A, R at level 50).
 (** The terms t and u are reducibly convertible at type A and level 0 in Γ, given the proof R that A is reducible *)
-Reserved Notation "[ Γ ||-<0> t ≅ u : A | R ]" (at level 0, Γ, t, u, A, R at level 50).
+Reserved Notation "[ Γ ||-<0> t ≅ u : A | R ]< l >" (at level 0, Γ, l, t, u, A, R at level 50).
 
 
 
 
 (** ** Validity notations *)
-Reserved Notation "[||-v Γ ]" (at level 0, Γ at level 50).
-Reserved Notation "[ Δ ||-v σ : Γ | VΓ | wfΔ ]" (at level 0, Δ, σ, Γ, VΓ, wfΔ at level 50).
-Reserved Notation "[ Δ ||-v σ ≅ σ' : Γ | VΓ | wfΔ | vσ ]" (at level 0, Δ, σ, σ', Γ, VΓ, wfΔ, vσ at level 50).
-Reserved Notation "[ Γ ||-v< k > A | VΓ ]" (at level 0, Γ, k , A, VΓ at level 50).
-Reserved Notation "[ P | Δ ||-v σ : Γ | wfΔ ]" (at level 0, P, Δ, σ, Γ, wfΔ at level 50).
-Reserved Notation "[ P | Δ ||-v σ ≅ σ' : Γ | wfΔ | vσ ]"  (at level 0, P, Δ, σ, σ', Γ, wfΔ, vσ at level 50).
-Reserved Notation "[ R | ||-v Γ ]"  (at level 0, R, Γ at level 50).
-Reserved Notation "[ R | Δ ||-v σ : Γ | RΓ | wfΔ ]"  (at level 0, R, Δ, σ, Γ, RΓ, wfΔ at level 50).
-Reserved Notation "[ R | Δ ||-v σ ≅ σ' : Γ | RΓ | wfΔ | vσ ]" (at level 0, R, Δ, σ, σ', Γ, RΓ, wfΔ, vσ at level 50).
-Reserved Notation "[ P | Γ ||-v< k > A ]"  (at level 0, P, Γ, k, A at level 50).
+Reserved Notation "[||-v Γ ]< l >" (at level 0, Γ, l at level 50).
+Reserved Notation "[ Δ ||-v σ : Γ | VΓ | wfΔ ]< l >" (at level 0, Δ, σ, Γ, l, VΓ, wfΔ at level 50).
+Reserved Notation "[ Δ ||-v σ ≅ σ' : Γ | VΓ | wfΔ | vσ ]< l >" (at level 0, Δ, σ, σ', Γ, l, VΓ, wfΔ, vσ at level 50).
+Reserved Notation "[ Γ ||-v< k > A | VΓ ]< l >" (at level 0, Γ, l, k , A, VΓ at level 50).
+Reserved Notation "[ P | Δ ||-v σ : Γ | wfΔ ]< l >" (at level 0, P, Δ, σ, Γ, l, wfΔ at level 50).
+Reserved Notation "[ P | Δ ||-v σ ≅ σ' : Γ | wfΔ | vσ ]< l >"  (at level 0, P, Δ, σ, σ', Γ, l, wfΔ, vσ at level 50).
+Reserved Notation "[ R | ||-v Γ ]< l >"  (at level 0, R, Γ, l at level 50).
+Reserved Notation "[ R | Δ ||-v σ : Γ | RΓ | wfΔ ]< l >"  (at level 0, R, Δ, σ, Γ, l, RΓ, wfΔ at level 50).
+Reserved Notation "[ R | Δ ||-v σ ≅ σ' : Γ | RΓ | wfΔ | vσ ]< l >" (at level 0, R, Δ, σ, σ', Γ, l, RΓ, wfΔ, vσ at level 50).
+Reserved Notation "[ P | Γ ||-v< k > A ]< l >"  (at level 0, P, Γ, l, l, k, A at level 50).
 
 (** LCon Notations *)
 Notation " ne £ b ::l l" := (wfLCons l ne b) (at level 40).
